Optimizations/ConditionalElimination.thy
@@ -6,10 +6,23 @@ theory ConditionalElimination
     Proofs.Stuttering
     Proofs.Form
     Proofs.Rewrites
+    Proofs.Bisimulation
 begin
 
+subsection \<open>Individual Elimination Rules\<close>
+text \<open>
+We introduce a TriState as in the Graal compiler to represent when static
+analysis can tell us information about the value of a boolean expression.
+Unknown = No information can be inferred
+KnownTrue/KnownFalse = We can infer the expression will always be true or false.
+\<close>
 datatype TriState = Unknown | KnownTrue | KnownFalse
 
+text \<open>
+The implies relation corresponds to the LogicNode.implies
+method from the compiler which attempts to infer when one
+logic nodes value can be inferred from a known logic node.
+\<close>
 inductive implies :: "IRGraph \<Rightarrow> IRNode \<Rightarrow> IRNode \<Rightarrow> TriState \<Rightarrow> bool"
   ("_ \<turnstile> _ & _ \<hookrightarrow> _") for g where
   eq_imp_less:
@@ -31,50 +44,174 @@ inductive implies :: "IRGraph \<Rightarrow> IRNode \<Rightarrow> IRNode \<Righta
   negate_true:
   "\<lbrakk>g \<turnstile> x & (kind g y) \<hookrightarrow> KnownFalse\<rbrakk> \<Longrightarrow> g \<turnstile> x & (NegateNode y) \<hookrightarrow> KnownTrue"
 
+
+text \<open>Total relation over partial implies relation\<close>
 inductive condition_implies :: "IRGraph \<Rightarrow> IRNode \<Rightarrow> IRNode \<Rightarrow> TriState \<Rightarrow> bool"
   ("_ \<turnstile> _ & _ \<rightharpoonup> _") for g where
   "\<lbrakk>\<not>(g \<turnstile> a & b \<hookrightarrow> imp)\<rbrakk> \<Longrightarrow> (g \<turnstile> a & b \<rightharpoonup> Unknown)" |
   "\<lbrakk>(g \<turnstile> a & b \<hookrightarrow> imp)\<rbrakk> \<Longrightarrow> (g \<turnstile> a & b \<rightharpoonup> imp)"
 
+text \<open>
+Proofs that the implies relation is correct with respect to the 
+existing evaluation semantics.
+\<close>
+(* TODO: I've broken this proof, the shows is not showing the writen this due to order of ops *)
+lemma implies_valid:
+  assumes "wff_graph g"
+  assumes "g \<turnstile> x & y \<rightharpoonup> imp"
+  assumes "g m \<turnstile> x \<mapsto> v1"
+  assumes "g m \<turnstile> y \<mapsto> v2"
+  shows "imp = KnownTrue \<longrightarrow> (val_to_bool v1 \<longrightarrow> val_to_bool v2) \<and>
+         imp = KnownFalse \<longrightarrow> (val_to_bool v1 \<longrightarrow> \<not>(val_to_bool v2))"
+proof (cases imp)
+  case Unknown
+  then show ?thesis
+    by simp
+next
+  case KnownTrue
+  have s: "g \<turnstile> x & y \<hookrightarrow> imp"
+    using assms(2) KnownTrue condition_implies.cases by blast
+  then show ?thesis
+  using assms proof (induct x y imp rule: implies.induct)
+    case (eq_imp_less x y)
+    then show ?case by simp
+  next
+    case (eq_imp_less_rev x y)
+    then show ?case by simp
+  next
+    case (less_imp_rev_less x y)
+    then show ?case by simp
+  next
+    case (less_imp_not_eq x y)
+    then show ?case by simp
+  next
+    case (less_imp_not_eq_rev x y)
+    then show ?case by simp
+  next
+    case (x_imp_x x1)
+    then show ?case using evalDet
+      using assms(2,3) by blast
+  next
+    case (negate_false x1)
+    then show ?case using evalDet
+      using assms(2,3) by blast
+  next
+    case (negate_true x y)
+    show ?case using negate_true.hyps(1)
+      by simp
+  qed
+next
+  case KnownFalse
+  have "g \<turnstile> x & y \<hookrightarrow> imp"
+    using KnownFalse assms(2) condition_implies.cases by blast
+  then show ?thesis
+  using assms proof (induct x y imp rule: implies.induct)
+    case (eq_imp_less x y)
+    obtain b xval where xval: "g m \<turnstile> (kind g x) \<mapsto> IntVal b xval"
+      using eq_imp_less.prems(3) by blast
+    then obtain yval where yval: "g m \<turnstile> (kind g y) \<mapsto> IntVal b yval"
+      using eq_imp_less.prems(3)
+      using evalDet by blast
+    have eqeval: "g m \<turnstile> (IntegerEqualsNode x y) \<mapsto> bool_to_val(xval = yval)"
+      using eval.IntegerEqualsNode
+      using xval yval by blast
+    have lesseval: "g m \<turnstile> (IntegerLessThanNode x y) \<mapsto> bool_to_val(xval < yval)"
+      using eval.IntegerLessThanNode
+      using xval yval by blast
+    have "xval = yval \<longrightarrow> \<not>(xval < yval)"
+      by blast
+    then show ?case
+      using eqeval lesseval
+      by (metis (full_types) "eq_imp_less.prems"(3) "eq_imp_less.prems"(4) bool_to_val.simps(2) evalDet val_to_bool.simps(1))
+  next
+    case (eq_imp_less_rev x y)
+    obtain b xval where xval: "g m \<turnstile> (kind g x) \<mapsto> IntVal b xval"
+      using eq_imp_less_rev.prems(3) by blast
+    then obtain yval where yval: "g m \<turnstile> (kind g y) \<mapsto> IntVal b yval"
+      using eq_imp_less_rev.prems(3)
+      using evalDet by blast
+    have eqeval: "g m \<turnstile> (IntegerEqualsNode x y) \<mapsto> bool_to_val(xval = yval)"
+      using eval.IntegerEqualsNode
+      using xval yval by blast
+    have lesseval: "g m \<turnstile> (IntegerLessThanNode y x) \<mapsto> bool_to_val(yval < xval)"
+      using eval.IntegerLessThanNode
+      using xval yval by blast
+    have "xval = yval \<longrightarrow> \<not>(yval < xval)"
+      by blast
+    then show ?case
+      using eqeval lesseval
+      by (metis (full_types) eq_imp_less_rev.prems(3) eq_imp_less_rev.prems(4) bool_to_val.simps(2) evalDet val_to_bool.simps(1))
+  next
+    case (less_imp_rev_less x y)
+    obtain b xval where xval: "g m \<turnstile> (kind g x) \<mapsto> IntVal b xval"
+      using less_imp_rev_less.prems(3) by blast
+    then obtain yval where yval: "g m \<turnstile> (kind g y) \<mapsto> IntVal b yval"
+      using less_imp_rev_less.prems(3)
+      using evalDet by blast
+    have lesseval: "g m \<turnstile> (IntegerLessThanNode x y) \<mapsto> bool_to_val(xval < yval)"
+      using eval.IntegerLessThanNode
+      using xval yval by blast
+    have revlesseval: "g m \<turnstile> (IntegerLessThanNode y x) \<mapsto> bool_to_val(yval < xval)"
+      using eval.IntegerLessThanNode
+      using xval yval by blast
+    have "xval < yval \<longrightarrow> \<not>(yval < xval)"
+      by simp
+    then show ?case
+      by (metis (full_types) bool_to_val.simps(2) evalDet less_imp_rev_less.prems(3,4) less_imp_rev_less.prems(3) lesseval revlesseval val_to_bool.simps(1))
+  next
+    case (less_imp_not_eq x y)
+    obtain b xval where xval: "g m \<turnstile> (kind g x) \<mapsto> IntVal b xval"
+      using less_imp_not_eq.prems(3) by blast
+    then obtain yval where yval: "g m \<turnstile> (kind g y) \<mapsto> IntVal b yval"
+      using less_imp_not_eq.prems(3)
+      using evalDet by blast
+    have eqeval: "g m \<turnstile> (IntegerEqualsNode x y) \<mapsto> bool_to_val(xval = yval)"
+      using eval.IntegerEqualsNode
+      using xval yval by blast
+    have lesseval: "g m \<turnstile> (IntegerLessThanNode x y) \<mapsto> bool_to_val(xval < yval)"
+      using eval.IntegerLessThanNode
+      using xval yval by blast
+    have "xval < yval \<longrightarrow> \<not>(xval = yval)"
+      by simp
+    then show ?case
+      by (metis (full_types) bool_to_val.simps(2) eqeval evalDet less_imp_not_eq.prems(3,4) less_imp_not_eq.prems(3) lesseval val_to_bool.simps(1))
+  next
+    case (less_imp_not_eq_rev x y)
+    obtain b xval where xval: "g m \<turnstile> (kind g x) \<mapsto> IntVal b xval"
+      using less_imp_not_eq_rev.prems(3) by blast
+    then obtain yval where yval: "g m \<turnstile> (kind g y) \<mapsto> IntVal b yval"
+      using less_imp_not_eq_rev.prems(3)
+      using evalDet by blast
+    have eqeval: "g m \<turnstile> (IntegerEqualsNode y x) \<mapsto> bool_to_val(yval = xval)"
+      using eval.IntegerEqualsNode
+      using xval yval by blast
+    have lesseval: "g m \<turnstile> (IntegerLessThanNode x y) \<mapsto> bool_to_val(xval < yval)"
+      using eval.IntegerLessThanNode
+      using xval yval by blast
+    have "xval < yval \<longrightarrow> \<not>(yval = xval)"
+      by simp
+    then show ?case
+      by (metis (full_types) bool_to_val.simps(2) eqeval evalDet less_imp_not_eq_rev.prems(3,4) less_imp_not_eq_rev.prems(3) lesseval val_to_bool.simps(1))
+  next
+    case (x_imp_x x1)
+    then show ?case by simp
+  next
+    case (negate_false x1)
+    then show ?case by simp
+  next
+    case (negate_true x1)
+    then show ?case by simp
+  qed
+qed
+
 lemma implies_true_valid:
+  assumes "wff_graph g"
   assumes "g \<turnstile> x & y \<rightharpoonup> imp"
   assumes "imp = KnownTrue"
   assumes "g m \<turnstile> x \<mapsto> v1"
   assumes "g m \<turnstile> y \<mapsto> v2"
   shows "val_to_bool v1 \<longrightarrow> val_to_bool v2"
-proof -
-  have s: "g \<turnstile> x & y \<hookrightarrow> imp"
-    using assms(1) assms(2) condition_implies.cases by blast
-
-then show ?thesis
-using assms proof (induct x y imp rule: implies.induct)
-  case (eq_imp_less x y)
-  then show ?case by simp
-next
-  case (eq_imp_less_rev x y)
-  then show ?case by simp
-next
-  case (less_imp_rev_less x y)
-  then show ?case by simp
-next
-  case (less_imp_not_eq x y)
-  then show ?case by simp
-next
-  case (less_imp_not_eq_rev x y)
-  then show ?case by simp
-next
-  case (x_imp_x x1)
-  then show ?case using evalDet
-    using assms(3) assms(4) by blast
-next
-  case (negate_false x1)
-  then show ?case using evalDet
-    using assms(3) assms(4) by blast
-next
-  case (negate_true x y)
-  show ?case using negate_true.hyps(1) sorry
-qed
-qed
+  using assms implies_valid sorry
 
 lemma implies_false_valid:
   assumes "wff_graph g"
@@ -83,116 +220,15 @@ lemma implies_false_valid:
   assumes "g m \<turnstile> x \<mapsto> v1"
   assumes "g m \<turnstile> y \<mapsto> v2"
   shows "val_to_bool v1 \<longrightarrow> \<not>(val_to_bool v2)"
-proof -
-  have "g \<turnstile> x & y \<hookrightarrow> imp"
-    using assms(2) assms(3) condition_implies.cases by blast
+  using assms implies_valid sorry
 
-then show ?thesis
-using assms proof (induct x y imp rule: implies.induct)
-  case (eq_imp_less x y)
-  obtain b xval where xval: "g m \<turnstile> (kind g x) \<mapsto> IntVal b xval"
-    using eq_imp_less.prems(4) by blast
-  then obtain yval where yval: "g m \<turnstile> (kind g y) \<mapsto> IntVal b yval"
-    using eq_imp_less.prems(4)
-    using evalDet by blast
-  have eqeval: "g m \<turnstile> (IntegerEqualsNode x y) \<mapsto> bool_to_val(xval = yval)"
-    using eval.IntegerEqualsNode
-    using xval yval by blast
-  have lesseval: "g m \<turnstile> (IntegerLessThanNode x y) \<mapsto> bool_to_val(xval < yval)"
-    using eval.IntegerLessThanNode
-    using xval yval by blast
-  have "xval = yval \<longrightarrow> \<not>(xval < yval)"
-    by blast
-  then show ?case
-    using eqeval lesseval
-    by (metis (full_types) "eq_imp_less.prems"(4) "eq_imp_less.prems"(5) bool_to_val.simps(2) evalDet val_to_bool.simps(1))
-next
-  case (eq_imp_less_rev x y)
-  obtain b xval where xval: "g m \<turnstile> (kind g x) \<mapsto> IntVal b xval"
-    using eq_imp_less_rev.prems(4) by blast
-  then obtain yval where yval: "g m \<turnstile> (kind g y) \<mapsto> IntVal b yval"
-    using eq_imp_less_rev.prems(4)
-    using evalDet by blast
-  have eqeval: "g m \<turnstile> (IntegerEqualsNode x y) \<mapsto> bool_to_val(xval = yval)"
-    using eval.IntegerEqualsNode
-    using xval yval by blast
-  have lesseval: "g m \<turnstile> (IntegerLessThanNode y x) \<mapsto> bool_to_val(yval < xval)"
-    using eval.IntegerLessThanNode
-    using xval yval by blast
-  have "xval = yval \<longrightarrow> \<not>(yval < xval)"
-    by blast
-  then show ?case
-    using eqeval lesseval
-    by (metis (full_types) eq_imp_less_rev.prems(4) eq_imp_less_rev.prems(5) bool_to_val.simps(2) evalDet val_to_bool.simps(1))
-next
-  case (less_imp_rev_less x y)
-  obtain b xval where xval: "g m \<turnstile> (kind g x) \<mapsto> IntVal b xval"
-    using less_imp_rev_less.prems(4) by blast
-  then obtain yval where yval: "g m \<turnstile> (kind g y) \<mapsto> IntVal b yval"
-    using less_imp_rev_less.prems(4)
-    using evalDet by blast
-  have lesseval: "g m \<turnstile> (IntegerLessThanNode x y) \<mapsto> bool_to_val(xval < yval)"
-    using eval.IntegerLessThanNode
-    using xval yval by blast
-  have revlesseval: "g m \<turnstile> (IntegerLessThanNode y x) \<mapsto> bool_to_val(yval < xval)"
-    using eval.IntegerLessThanNode
-    using xval yval by blast
-  have "xval < yval \<longrightarrow> \<not>(yval < xval)"
-    by simp
-  then show ?case
-    by (metis (full_types) bool_to_val.simps(2) evalDet less_imp_rev_less.prems(4) less_imp_rev_less.prems(5) lesseval revlesseval val_to_bool.simps(1))
-next
-  case (less_imp_not_eq x y)
-  obtain b xval where xval: "g m \<turnstile> (kind g x) \<mapsto> IntVal b xval"
-    using less_imp_not_eq.prems(4) by blast
-  then obtain yval where yval: "g m \<turnstile> (kind g y) \<mapsto> IntVal b yval"
-    using less_imp_not_eq.prems(4)
-    using evalDet by blast
-  have eqeval: "g m \<turnstile> (IntegerEqualsNode x y) \<mapsto> bool_to_val(xval = yval)"
-    using eval.IntegerEqualsNode
-    using xval yval by blast
-  have lesseval: "g m \<turnstile> (IntegerLessThanNode x y) \<mapsto> bool_to_val(xval < yval)"
-    using eval.IntegerLessThanNode
-    using xval yval by blast
-  have "xval < yval \<longrightarrow> \<not>(xval = yval)"
-    by simp
-  then show ?case
-    by (metis (full_types) bool_to_val.simps(2) eqeval evalDet less_imp_not_eq.prems(4) less_imp_not_eq.prems(5) lesseval val_to_bool.simps(1))
-next
-  case (less_imp_not_eq_rev x y)
-  obtain b xval where xval: "g m \<turnstile> (kind g x) \<mapsto> IntVal b xval"
-    using less_imp_not_eq_rev.prems(4) by blast
-  then obtain yval where yval: "g m \<turnstile> (kind g y) \<mapsto> IntVal b yval"
-    using less_imp_not_eq_rev.prems(4)
-    using evalDet by blast
-  have eqeval: "g m \<turnstile> (IntegerEqualsNode y x) \<mapsto> bool_to_val(yval = xval)"
-    using eval.IntegerEqualsNode
-    using xval yval by blast
-  have lesseval: "g m \<turnstile> (IntegerLessThanNode x y) \<mapsto> bool_to_val(xval < yval)"
-    using eval.IntegerLessThanNode
-    using xval yval by blast
-  have "xval < yval \<longrightarrow> \<not>(yval = xval)"
-    by simp
-  then show ?case
-    by (metis (full_types) bool_to_val.simps(2) eqeval evalDet less_imp_not_eq_rev.prems(4) less_imp_not_eq_rev.prems(5) lesseval val_to_bool.simps(1))
-next
-  case (x_imp_x x1)
-  then show ?case by simp
-next
-  case (negate_false x1)
-  then show ?case using implies_true_valid sorry
-next
-  case (negate_true x1)
-  then show ?case by simp
-qed
-qed
+text \<open>
+The following relation corresponds to the UnaryOpLogicNode.tryFold
+and BinaryOpLogicNode.tryFold methods and their associated concrete implementations.
 
-fun alwaysDistinct :: "Stamp \<Rightarrow> Stamp \<Rightarrow> bool" where
-  "alwaysDistinct stamp1 stamp2 = is_stamp_empty (join stamp1 stamp2)"
-
-fun neverDistinct :: "Stamp \<Rightarrow> Stamp \<Rightarrow> bool" where
-  "neverDistinct stamp1 stamp2 = (asConstant stamp1 = asConstant stamp2 \<and> asConstant stamp1 \<noteq> UndefVal)"
-
+The relation determines if a logic operation can be shown true or false
+through the stamp typing information.
+\<close>
 inductive tryFold :: "IRNode \<Rightarrow> (ID \<Rightarrow> Stamp) \<Rightarrow> TriState \<Rightarrow> bool"
   where
   "\<lbrakk>alwaysDistinct (stamps x) (stamps y)\<rbrakk> 
@@ -208,112 +244,143 @@ inductive tryFold :: "IRNode \<Rightarrow> (ID \<Rightarrow> Stamp) \<Rightarrow
     stpi_lower (stamps x) \<ge> stpi_upper (stamps y)\<rbrakk> 
     \<Longrightarrow> tryFold (IntegerLessThanNode x y) stamps KnownFalse"
 
-lemma asConstantEval:
-  assumes "wff_stamps g"
-  assumes "asConstant (stamp g nid) = val"
-  assumes "val \<noteq> UndefVal"
-  assumes "g m \<turnstile> (kind g nid) \<mapsto> v"
-  shows "v = val"
-proof -
-  have "\<exists>b l h. stamp g nid = (IntegerStamp b l h)"
-    using assms(2,3) asConstant.elims by (cases "stamp g nid"; auto)
-  then obtain b l h where "stamp g nid = (IntegerStamp b l h)"
-    by blast
-  then have "l = h"
-    using asConstant.simps(1) assms(2) assms(3) by presburger
-  then have "{x . valid_value (stamp g nid) x} = {IntVal b l}"
-    using assms(2) assms(3) int_valid_range
-    using \<open>stamp g nid = IntegerStamp b l h\<close> by force
-  then show ?thesis using assms(1)
-    using \<open>l = h\<close> \<open>stamp g nid = IntegerStamp b l h\<close> assms(2) assms(4) by fastforce
-qed
 
+text \<open>
+Proofs that show that when the stamp lookup function is well-formed,
+the tryFold relation correctly predicts the output value with respect to
+our evaluation semantics.
+\<close>
 lemma tryFoldIntegerEqualsAlwaysDistinct:
-  assumes "wff_stamps g"
+  assumes "wff_stamp g stamps"
   assumes "kind g nid = (IntegerEqualsNode x y)"
   assumes "g m \<turnstile> (kind g nid) \<mapsto> v"
-  assumes "alwaysDistinct (stamp g x) (stamp g y)"
+  assumes "alwaysDistinct (stamps x) (stamps y)"
   shows "v = IntVal 1 0"
   using assms eval.IntegerEqualsNode join_unequal alwaysDistinct.simps
-  by (smt IntegerEqualsNodeE NoNodeE bool_to_val.simps(2) ids_some wff_stamps.simps)
+  by (smt (verit, best) IntegerEqualsNodeE bool_to_val.simps(2) eval_in_ids wff_stamp.elims(2))
 
 lemma tryFoldIntegerEqualsNeverDistinct:
-  assumes "wff_stamps g"
+  assumes "wff_stamp g stamps"
   assumes "kind g nid = (IntegerEqualsNode x y)"
   assumes "g m \<turnstile> (kind g nid) \<mapsto> v"
-  assumes "neverDistinct (stamp g x) (stamp g y)"
+  assumes "neverDistinct (stamps x) (stamps y)"
   shows "v = IntVal 1 1"
-  using assms asConstantEval neverDistinct.simps
-  by (smt IntegerEqualsNodeE Value.inject(1) bool_to_val.simps(1))
+  using assms neverDistinctEqual IntegerEqualsNodeE
+  by (smt (verit, ccfv_threshold) Value.inject(1) bool_to_val.simps(1) eval_in_ids wff_stamp.simps)
 
 lemma tryFoldIntegerLessThanTrue:
-  assumes "wff_stamps g"
+  assumes "wff_stamp g stamps"
   assumes "kind g nid = (IntegerLessThanNode x y)"
   assumes "g m \<turnstile> (kind g nid) \<mapsto> v"
-  assumes "stpi_upper (stamp g x) < stpi_lower (stamp g y)"
+  assumes "stpi_upper (stamps x) < stpi_lower (stamps y)"
   shows "v = IntVal 1 1"
-  sorry
+proof -
+  have stamp_type: "is_IntegerStamp (stamps x)"
+    by (metis IntegerLessThanNodeE Stamp.disc(2) Value.distinct(9) assms(1) assms(2) assms(3) eval_in_ids valid_value.elims(2) valid_value.simps(4) wff_stamp.elims(2))
+  obtain xval b where xval: "g m \<turnstile> kind g x \<mapsto> IntVal b xval"
+    using assms(2,3) eval.IntegerLessThanNode by auto
+  obtain yval b where yval: "g m \<turnstile> kind g y \<mapsto> IntVal b yval"
+    using assms(2,3) eval.IntegerLessThanNode by auto
+  have "is_IntegerStamp (stamps x) \<and> is_IntegerStamp (stamps y)"
+    using assms(4)
+    by (metis stamp_type Stamp.disc(2) Value.distinct(1) Value.distinct(9) assms(1) eval_in_ids valid_value.elims(2) wff_stamp.simps yval)
+  then have "xval < yval"
+    using boundsNoOverlap xval yval assms(1,4)
+    using eval_in_ids wff_stamp.elims(2)
+    by metis
+  then show ?thesis
+    by (metis (full_types) IntegerLessThanNodeE Value.sel(3) assms(2) assms(3) bool_to_val.simps(1) evalDet xval yval)
+qed
 
 lemma tryFoldIntegerLessThanFalse:
-  assumes "wff_stamps g"
+  assumes "wff_stamp g stamps"
   assumes "kind g nid = (IntegerLessThanNode x y)"
   assumes "g m \<turnstile> (kind g nid) \<mapsto> v"
-  assumes "stpi_lower (stamp g x) \<ge> stpi_upper (stamp g y)"
+  assumes "stpi_lower (stamps x) \<ge> stpi_upper (stamps y)"
   shows "v = IntVal 1 0"
-  sorry
+  proof -
+  have stamp_type: "is_IntegerStamp (stamps x)"
+    by (metis IntegerLessThanNodeE Stamp.disc(2) Value.distinct(9) assms(1) assms(2) assms(3) eval_in_ids valid_value.elims(2) valid_value.simps(4) wff_stamp.elims(2))
+  obtain xval b where xval: "g m \<turnstile> kind g x \<mapsto> IntVal b xval"
+    using assms(2,3) eval.IntegerLessThanNode by auto
+  obtain yval b where yval: "g m \<turnstile> kind g y \<mapsto> IntVal b yval"
+    using assms(2,3) eval.IntegerLessThanNode by auto
+  have "is_IntegerStamp (stamps x) \<and> is_IntegerStamp (stamps y)"
+    using assms(4)
+    by (metis stamp_type Stamp.disc(2) Value.distinct(1) Value.distinct(9) assms(1) eval_in_ids valid_value.elims(2) wff_stamp.simps yval)
+  then have "\<not>(xval < yval)"
+    using boundsAlwaysOverlap xval yval assms(1,4)
+    using eval_in_ids wff_stamp.elims(2)
+    by metis
+  then show ?thesis
+    by (smt (verit, best) IntegerLessThanNodeE Value.inject(1) assms(2) assms(3) bool_to_val.simps(2) evalDet xval yval)
+qed
 
 theorem tryFoldProofTrue:
-  assumes "wff_stamps g"
-  assumes "tryFold (kind g nid) (stamp g) tristate"
+  assumes "wff_stamp g stamps"
+  assumes "tryFold (kind g nid) stamps tristate"
   assumes "tristate = KnownTrue"
   assumes "g m \<turnstile> kind g nid \<mapsto> v"
   shows "val_to_bool v"
-  using assms(2) proof (induction "kind g nid" "stamp g" tristate rule: tryFold.induct)
-case (1 x y)
-  then show ?case using tryFoldIntegerEqualsAlwaysDistinct assms(1,4)
-    by (smt (verit, del_insts) IRNode.distinct(949) TriState.simps(6) Value.inject(1) assms(2) assms(3) tryFold.cases tryFoldIntegerEqualsNeverDistinct)
+  using assms(2) proof (induction "kind g nid" stamps tristate rule: tryFold.induct)
+case (1 stamps x y)
+  then show ?case using tryFoldIntegerEqualsAlwaysDistinct assms
+    by (smt (verit, best) IRNode.distinct(949) TriState.distinct(5) tryFold.cases tryFoldIntegerEqualsNeverDistinct val_to_bool.simps(1))
 next
-  case (2 x y)
-  then show ?case using tryFoldIntegerEqualsAlwaysDistinct assms(1,4)
-    by (metis tryFoldIntegerEqualsNeverDistinct val_to_bool.simps(1) zero_neq_one)
+  case (2 stamps x y)
+  then show ?case using tryFoldIntegerEqualsAlwaysDistinct assms
+    by (smt (verit) IRNode.distinct(949) TriState.distinct(5) tryFold.cases tryFoldIntegerEqualsNeverDistinct val_to_bool.simps(1))
 next
-case (3 x y)
-  then show ?case using tryFoldIntegerLessThanTrue assms(1,4)
-    by (metis val_to_bool.simps(1) zero_neq_one)
+  case (3 stamps x y)
+  then show ?case using tryFoldIntegerLessThanTrue assms
+    by (smt (verit, best) IRNode.simps(994) TriState.simps(6) tryFold.cases val_to_bool.simps(1))
 next
-case (4 x y)
-  then show ?case using assms(3)
-    by (smt (verit, best) TriState.distinct(5) Value.inject(1) assms(1) assms(2) assms(4) tryFold.cases tryFoldIntegerEqualsNeverDistinct tryFoldIntegerLessThanFalse tryFoldIntegerLessThanTrue)
+case (4 stamps x y)
+  then show ?case using tryFoldIntegerLessThanFalse assms
+    by (smt (verit, best) IRNode.simps(994) TriState.simps(6) tryFold.simps tryFoldIntegerLessThanTrue val_to_bool.simps(1))
 qed
 
 theorem tryFoldProofFalse:
-  assumes "wff_stamps g"
-  assumes "tryFold (kind g nid) (stamp g) tristate"
+  assumes "wff_stamp g stamps"
+  assumes "tryFold (kind g nid) stamps tristate"
   assumes "tristate = KnownFalse"
   assumes "g m \<turnstile> (kind g nid) \<mapsto> v"
   shows "\<not>(val_to_bool v)"
-using assms(2) proof (induction "kind g nid" "stamp g" tristate rule: tryFold.induct)
-case (1 x y)
-  then show ?case using tryFoldIntegerEqualsAlwaysDistinct assms(1,4)
-    by (metis val_to_bool.simps(1))
+using assms(2) proof (induction "kind g nid" stamps tristate rule: tryFold.induct)
+case (1 stamps x y)
+  then show ?case using tryFoldIntegerEqualsAlwaysDistinct assms
+    by (smt (verit, best) IRNode.distinct(949) TriState.distinct(5) Value.inject(1) tryFold.cases val_to_bool.elims(2))
 next
-case (2 x y)
-  then show ?case using tryFoldIntegerEqualsNeverDistinct assms(1,4)
-    by (smt (verit, best) IRNode.distinct(949) TriState.distinct(5) Value.inject(1) assms(2) assms(3) tryFold.cases tryFoldIntegerEqualsAlwaysDistinct)
+case (2 stamps x y)
+  then show ?case using tryFoldIntegerEqualsNeverDistinct assms
+    by (smt (verit, best) IRNode.distinct(949) TriState.distinct(5) Value.inject(1) tryFold.cases tryFoldIntegerEqualsAlwaysDistinct val_to_bool.elims(2))
 next
-case (3 x y)
-  then show ?case using tryFoldIntegerLessThanTrue assms(1,4)
-    by (smt (verit, best) IRNode.simps(993) TriState.simps(6) Value.inject(1) assms(2) assms(3) tryFold.cases tryFoldIntegerLessThanFalse)
+  case (3 stamps x y)
+  then show ?case using tryFoldIntegerLessThanTrue assms
+    by (smt (verit, best) TriState.distinct(5) tryFold.cases tryFoldIntegerEqualsAlwaysDistinct tryFoldIntegerLessThanFalse val_to_bool.simps(1))
 next
-  case (4 x y)
-  then show ?case using tryFoldIntegerLessThanFalse assms(1,4)
-    by (metis val_to_bool.simps(1))
+  case (4 stamps x y)
+  then show ?case using tryFoldIntegerLessThanFalse assms
+    by (smt (verit, best) TriState.distinct(5) tryFold.cases tryFoldIntegerEqualsAlwaysDistinct val_to_bool.simps(1))
 qed
+
+
 
 inductive_cases StepE:
   "g \<turnstile> (nid,m,h) \<rightarrow> (nid',m',h)"
 
+text \<open>
+Perform conditional elimination rewrites on the graph for a particular node.
 
+In order to determine conditional eliminations appropriately the rule needs two
+data structures produced by static analysis.
+The first parameter is the set of IRNodes that we know result in a true value
+when evaluated.
+The second parameter is a mapping from node identifiers to the flow-sensitive stamp.
+
+The relation transforms the third parameter to the fifth parameter for a node identifier
+which represents the fourth parameter.
+\<close>
 inductive ConditionalEliminationStep :: 
   "IRNode set \<Rightarrow> (ID \<Rightarrow> Stamp) \<Rightarrow> IRGraph \<Rightarrow> ID \<Rightarrow> IRGraph \<Rightarrow> bool" where
   impliesTrue:
@@ -344,15 +411,37 @@ inductive ConditionalEliminationStep ::
     g' = constantCondition False ifcond (kind g ifcond) g
     \<rbrakk> \<Longrightarrow> ConditionalEliminationStep conds stamps g ifcond g'"
 
+
 code_pred (modes: i \<Rightarrow> i \<Rightarrow> i \<Rightarrow> i \<Rightarrow> o \<Rightarrow> bool) ConditionalEliminationStep .
 
+thm ConditionalEliminationStep.equation
 
+subsection \<open>Control-flow Graph Traversal\<close>
 
-fun nextEdge :: "ID set \<Rightarrow> ID \<Rightarrow> IRGraph \<Rightarrow> ID option" where
+type_synonym Seen = "ID set"
+type_synonym Conditions = "IRNode list"
+type_synonym StampFlow = "(ID \<Rightarrow> Stamp) list"
+
+text \<open>
+nextEdge helps determine which node to traverse next by returning the first successor
+edge that isn't in the set of already visited nodes.
+If there is not an appropriate successor, None is returned instead.
+\<close>
+fun nextEdge :: "Seen \<Rightarrow> ID \<Rightarrow> IRGraph \<Rightarrow> ID option" where
   "nextEdge seen nid g = 
     (let nids = (filter (\<lambda>nid'. nid' \<notin> seen) (successors_of (kind g nid))) in 
      (if length nids > 0 then Some (hd nids) else None))"
 
+text \<open>
+pred determines which node, if any, acts as the predecessor of another.
+
+Merge nodes represent a special case where-in the predecessor exists as
+an input edge of the merge node, to simplify the traversal we treat only
+the first input end node as the predecessor, ignoring that multiple nodes
+may act as a successor.
+
+For all other nodes, the predecessor is the first element of the predecessors set.
+Note that in a well-formed graph there should only be one element in the predecessor set.\<close>
 fun pred :: "IRGraph \<Rightarrow> ID \<Rightarrow> ID option" where
   "pred g nid = (case kind g nid of
     (MergeNode ends _ _) \<Rightarrow> Some (hd ends) |
@@ -363,11 +452,15 @@ fun pred :: "IRGraph \<Rightarrow> ID \<Rightarrow> ID option" where
       )
   )"
 
-type_synonym Seen = "ID set"
-type_synonym Conditions = "IRNode list"
-type_synonym StampFlow = "(ID \<Rightarrow> Stamp) list"
 
-(* mimics the stamp updates from registerNewCondition *)
+text \<open>
+When the basic block of an if statement is entered, we know that the condition of the
+preceding if statement must be true.
+As in the GraalVM compiler, we introduce the registerNewCondition funciton which roughly
+corresponds to the ConditionalEliminationPhase.registerNewCondition.
+This method updates the flow-sensitive stamp information based on the condition which
+we know must be true. 
+\<close>
 fun registerNewCondition :: "IRGraph \<Rightarrow> IRNode \<Rightarrow> (ID \<Rightarrow> Stamp) \<Rightarrow> (ID \<Rightarrow> Stamp)" where
   (* constrain equality by joining the stamps *)
   "registerNewCondition g (IntegerEqualsNode x y) stamps =
@@ -378,19 +471,29 @@ fun hdOr :: "'a list \<Rightarrow> 'a \<Rightarrow> 'a" where
   "hdOr (x # xs) de = x" |
   "hdOr [] de = de"
 
-definition noFlow :: "(ID \<Rightarrow> Stamp)" where
-  "noFlow = (\<lambda>id. IllegalStamp)"
+text \<open>
+The Step relation is a small-step traversal of the graph which handles transitions between
+individual nodes of the graph.
 
+It relates a pairs of tuple of the current node, the set of seen nodes, 
+the always true stack of IfNode conditions, and the flow-sensitive stamp information.
+\<close>
 inductive Step 
   :: "IRGraph \<Rightarrow> (ID \<times> Seen \<times> Conditions \<times> StampFlow) \<Rightarrow> (ID \<times> Seen \<times> Conditions \<times> StampFlow) option \<Rightarrow> bool"
   for g where
-  (* Hit a BeginNode
-     1. nid' will be the successor of the begin node
-     2. Find the first and only predecessor
-     3. Extract condition from pred (pred is assumed IfNode)
+  \<comment> \<open>
+  Hit a BeginNode with an IfNode predecessor which represents
+  the start of a basic block for the IfNode.
+     1. nid' will be the successor of the begin node.
+     2. Find the first and only predecessor.
+     3. Extract condition from the preceding IfNode.
      4. Negate condition if the begin node is second branch
-     5. Add condition or negated condition to stack
-  *)  
+        (we've taken the else branch of the condition)
+     5. Add the condition or the negated condition to stack
+     6. Perform any stamp updates based on the condition using
+        the registerNewCondition function and place them on the
+        top of the stack of stamp information
+  \<close>
   "\<lbrakk>kind g nid = BeginNode nid';
 
     nid \<notin> seen;
@@ -406,10 +509,11 @@ inductive Step
     flow' = registerNewCondition g (kind g cond) (hdOr flow (stamp g))\<rbrakk>
    \<Longrightarrow> Step g (nid, seen, conds, flow) (Some (nid', seen', conds', flow' # flow))" |
 
-  (* Hit an EndNode
+  \<comment> \<open>
+  Hit an EndNode
      1. nid' will be the usage of EndNode
-     2. pop the conditions stack
-  *)
+     2. pop the conditions and stamp stack
+  \<close>
   "\<lbrakk>kind g nid = EndNode;
 
     nid \<notin> seen;
@@ -421,7 +525,7 @@ inductive Step
     flow' = tl flow\<rbrakk>
    \<Longrightarrow> Step g (nid, seen, conds, flow) (Some (nid', seen', conds', flow'))" |
 
-  (* We can find a successor edge that is not in seen, go there *)
+  \<comment> \<open>We can find a successor edge that is not in seen, go there\<close>
   "\<lbrakk>\<not>(is_EndNode (kind g nid));
     \<not>(is_BeginNode (kind g nid));
 
@@ -431,7 +535,7 @@ inductive Step
     Some nid' = nextEdge seen' nid g\<rbrakk>
    \<Longrightarrow> Step g (nid, seen, conds, flow) (Some (nid', seen', conds, flow))" |
 
-  (* We can cannot find a successor edge that is not in seen, give back None *)
+  \<comment> \<open>We can cannot find a successor edge that is not in seen, give back None\<close>
   "\<lbrakk>\<not>(is_EndNode (kind g nid));
     \<not>(is_BeginNode (kind g nid));
 
@@ -441,46 +545,52 @@ inductive Step
     None = nextEdge seen' nid g\<rbrakk>
     \<Longrightarrow> Step g (nid, seen, conds, flow) None" |
 
-  (* We've already seen this node, give back None *)
+  \<comment> \<open>We've already seen this node, give back None\<close>
   "\<lbrakk>nid \<in> seen\<rbrakk> \<Longrightarrow> Step g (nid, seen, conds, flow) None"
 
 code_pred (modes: i \<Rightarrow> i \<Rightarrow> o \<Rightarrow> bool) Step .
 
+
+text \<open>
+The ConditionalEliminationPhase relation is responsible for combining
+the individual traversal steps from the Step relation and the optimizations
+from the ConditionalEliminationStep relation to perform a transformation of the
+whole graph.
+\<close>
 inductive ConditionalEliminationPhase 
   :: "IRGraph \<Rightarrow> (ID \<times> Seen \<times> Conditions \<times> StampFlow) \<Rightarrow> IRGraph \<Rightarrow> bool" where
 
-  (* Can do a step and optimise for the current nid *)
+  \<comment> \<open>Can do a step and optimise for the current node\<close>
   "\<lbrakk>Step g (nid, seen, conds, flow) (Some (nid', seen', conds', flow'));
     ConditionalEliminationStep (set conds) (hdOr flow (stamp g)) g nid g';
     
     ConditionalEliminationPhase g' (nid', seen', conds', flow') g''\<rbrakk>
     \<Longrightarrow> ConditionalEliminationPhase g (nid, seen, conds, flow) g''" |
 
-  (* Can do a step, matches whether optimised or not causing non-determinism
-     Need to find a way to negate ConditionalEliminationStep *)
+  \<comment> \<open>Can do a step, matches whether optimised or not causing non-determinism
+      We need to find a way to negate ConditionalEliminationStep\<close>
   "\<lbrakk>Step g (nid, seen, conds, flow) (Some (nid', seen', conds', flow'));
     
     ConditionalEliminationPhase g (nid', seen', conds', flow') g'\<rbrakk>
     \<Longrightarrow> ConditionalEliminationPhase g (nid, seen, conds, flow) g'" |
 
-  (* Can't do a step but there is a predecessor we can backtrace to *)
+  \<comment> \<open>Can't do a step but there is a predecessor we can backtrace to\<close>
   "\<lbrakk>Step g (nid, seen, conds, flow) None;
     Some nid' = pred g nid;
     seen' = {nid} \<union> seen;
     ConditionalEliminationPhase g (nid', seen', conds, flow) g'\<rbrakk>
     \<Longrightarrow> ConditionalEliminationPhase g (nid, seen, conds, flow) g'" |
 
-  (* Can't do a step and have no predecessors do terminate *)
+  \<comment> \<open>Can't do a step and have no predecessors so terminate\<close>
   "\<lbrakk>Step g (nid, seen, conds, flow) None;
     None = pred g nid\<rbrakk>
     \<Longrightarrow> ConditionalEliminationPhase g (nid, seen, conds, flow) g"
 
+code_pred (modes: i \<Rightarrow> i \<Rightarrow> o \<Rightarrow> bool) ConditionalEliminationPhase .
 
-code_pred (modes: i \<Rightarrow> i \<Rightarrow> o \<Rightarrow> bool) 
-  ConditionalEliminationPhase .
 
-inductive ConditionalEliminationPhaseWithTrace
-  :: "IRGraph \<Rightarrow> (ID \<times> Seen \<times> Conditions \<times> StampFlow) \<Rightarrow> ID list \<Rightarrow> IRGraph \<Rightarrow> ID list \<Rightarrow> Conditions \<Rightarrow> bool" where
+inductive ConditionalEliminationPhaseWithTrace\<^marker>\<open>tag invisible\<close>
+  :: "IRGraph \<Rightarrow> (ID \<times> Seen \<times> Conditions \<times> StampFlow) \<Rightarrow> ID list \<Rightarrow> IRGraph \<Rightarrow> ID list \<Rightarrow> Conditions \<Rightarrow> bool" where\<^marker>\<open>tag invisible\<close>
 
   (* Can do a step and optimise for the current nid *)
   "\<lbrakk>Step g (nid, seen, conds, flow) (Some (nid', seen', conds', flow'));
@@ -508,199 +618,7 @@ inductive ConditionalEliminationPhaseWithTrace
     None = pred g nid\<rbrakk>
     \<Longrightarrow> ConditionalEliminationPhaseWithTrace g (nid, seen, conds, flow) t g (nid # t) conds"
 
-
-code_pred (modes: i \<Rightarrow> i \<Rightarrow> i \<Rightarrow> o \<Rightarrow> o \<Rightarrow> o \<Rightarrow> bool) 
-  ConditionalEliminationPhaseWithTrace .
-
-definition ConditionalEliminationTest1_test1Snippet_initial :: IRGraph where
-  "ConditionalEliminationTest1_test1Snippet_initial = irgraph [
-  (0, (StartNode  (Some 2) 7), VoidStamp),
-  (1, (ParameterNode 0), IntegerStamp 32 (-2147483648) (2147483647)),
-  (2, (FrameState []  None None None), IllegalStamp),
-  (3, (ConstantNode (IntVal 32 (0))), IntegerStamp 32 (0) (0)),
-  (4, (IntegerEqualsNode 1 3), VoidStamp),
-  (5, (BeginNode 39), VoidStamp),
-  (6, (BeginNode 12), VoidStamp),
-  (7, (IfNode 4 6 5), VoidStamp),
-  (8, (ConstantNode (IntVal 32 (5))), IntegerStamp 32 (5) (5)),
-  (9, (IntegerEqualsNode 1 8), VoidStamp),
-  (10, (BeginNode 16), VoidStamp),
-  (11, (BeginNode 14), VoidStamp),
-  (12, (IfNode 9 11 10), VoidStamp),
-  (13, (ConstantNode (IntVal 32 (100))), IntegerStamp 32 (100) (100)),
-  (14, (StoreFieldNode 14 ''org.graalvm.compiler.core.test.ConditionalEliminationTestBase::sink2'' 13  (Some 15)  None 18), VoidStamp),
-  (15, (FrameState []  None None None), IllegalStamp),
-  (16, (EndNode), VoidStamp),
-  (17, (MergeNode  [16, 18]  (Some 19) 24), VoidStamp),
-  (18, (EndNode), VoidStamp),
-  (19, (FrameState []  None None None), IllegalStamp),
-  (20, (ConstantNode (IntVal 32 (101))), IntegerStamp 32 (101) (101)),
-  (21, (IntegerLessThanNode 1 20), VoidStamp),
-  (22, (BeginNode 30), VoidStamp),
-  (23, (BeginNode 25), VoidStamp),
-  (24, (IfNode 21 23 22), VoidStamp),
-  (25, (EndNode), VoidStamp),
-  (26, (MergeNode  [25, 27, 34]  (Some 35) 43), VoidStamp),
-  (27, (EndNode), VoidStamp),
-  (28, (BeginNode 32), VoidStamp),
-  (29, (BeginNode 27), VoidStamp),
-  (30, (IfNode 4 28 29), VoidStamp),
-  (31, (ConstantNode (IntVal 32 (200))), IntegerStamp 32 (200) (200)),
-  (32, (StoreFieldNode 32 ''org.graalvm.compiler.core.test.ConditionalEliminationTest1::sink3'' 31  (Some 33)  None 34), VoidStamp),
-  (33, (FrameState []  None None None), IllegalStamp),
-  (34, (EndNode), VoidStamp),
-  (35, (FrameState []  None None None), IllegalStamp),
-  (36, (ConstantNode (IntVal 32 (2))), IntegerStamp 32 (2) (2)),
-  (37, (IntegerEqualsNode 1 36), VoidStamp),
-  (38, (BeginNode 45), VoidStamp),
-  (39, (EndNode), VoidStamp),
-  (40, (MergeNode  [39, 41, 47]  (Some 48) 49), VoidStamp),
-  (41, (EndNode), VoidStamp),
-  (42, (BeginNode 41), VoidStamp),
-  (43, (IfNode 37 42 38), VoidStamp),
-  (44, (ConstantNode (IntVal 32 (1))), IntegerStamp 32 (1) (1)),
-  (45, (StoreFieldNode 45 ''org.graalvm.compiler.core.test.ConditionalEliminationTestBase::sink1'' 44  (Some 46)  None 47), VoidStamp),
-  (46, (FrameState []  None None None), IllegalStamp),
-  (47, (EndNode), VoidStamp),
-  (48, (FrameState []  None None None), IllegalStamp),
-  (49, (StoreFieldNode 49 ''org.graalvm.compiler.core.test.ConditionalEliminationTestBase::sink0'' 3  (Some 50)  None 51), VoidStamp),
-  (50, (FrameState []  None None None), IllegalStamp),
-  (51, (ReturnNode  None  None), VoidStamp)
-  ]"
-values "{g' . ConditionalEliminationPhase ConditionalEliminationTest1_test1Snippet_initial (0, {}, [], []) g'}"
-
-
-definition exAlwaysDistinct :: "IRGraph" where
-  "exAlwaysDistinct = irgraph [
-    (0, (StartNode (None) (4)), VoidStamp),
-    (1, (ParameterNode (0)), IntegerStamp 32 (1) (2)),
-    (2, (ParameterNode (1)), IntegerStamp 32 (3) (4)),
-    (3, (IntegerEqualsNode (1) (2)), default_stamp),
-    (4, (IfNode (3) (5) (6)), VoidStamp),
-    (5, (BeginNode 7), VoidStamp),
-    (6, (BeginNode 8), VoidStamp),
-    (7, (EndNode), VoidStamp),
-    (8, (EndNode), VoidStamp),
-    (9, (MergeNode [7, 8] None 11), VoidStamp),
-    (10, (ValuePhiNode 10 [1, 2] 9), VoidStamp),
-    (11, (ReturnNode ((Some 10)) (None)), default_stamp)]"
-
-values "{g' . ConditionalEliminationPhase exAlwaysDistinct (0, {}, [], []) g'}"
-
-
-definition exNeverDistinct :: "IRGraph" where
-  "exNeverDistinct = irgraph [
-    (0, (StartNode (None) (4)), VoidStamp),
-    (1, (ParameterNode (0)), IntegerStamp 32 (1) (1)),
-    (2, (ParameterNode (1)), IntegerStamp 32 (1) (1)),
-    (3, (IntegerEqualsNode (1) (2)), default_stamp),
-    (4, (IfNode (3) (5) (6)), VoidStamp),
-    (5, (BeginNode 7), VoidStamp),
-    (6, (BeginNode 8), VoidStamp),
-    (7, (EndNode), VoidStamp),
-    (8, (EndNode), VoidStamp),
-    (9, (MergeNode [7, 8] None 11), VoidStamp),
-    (10, (ValuePhiNode 10 [1, 2] 9), VoidStamp),
-    (11, (ReturnNode ((Some 10)) (None)), default_stamp)]"
-values "{g' . ConditionalEliminationPhase exNeverDistinct (0, {}, [], []) g'}"
-
-definition exImpliesElim :: "IRGraph" where
-  "exImpliesElim = irgraph [
-    (0, (StartNode (None) (4)), VoidStamp),
-    (1, (ParameterNode (0)), default_stamp),
-    (2, (ParameterNode (1)), default_stamp),
-    (3, (IntegerEqualsNode (1) (2)), default_stamp),
-    (4, (IfNode (3) (5) (6)), VoidStamp),
-    (5, (BeginNode (9)), VoidStamp),
-    (6, (BeginNode (7)), VoidStamp),
-    (7, (EndNode), VoidStamp),
-    (8, (IntegerLessThanNode (1) (2)), default_stamp),
-    (9, (IfNode (8) (10) (11)), default_stamp),
-    (10, (BeginNode 12), VoidStamp),
-    (11, (BeginNode 13), VoidStamp),
-    (12, (EndNode), VoidStamp),
-    (13, (EndNode), VoidStamp),
-    (14, (MergeNode [12, 13] None 15), VoidStamp),
-    (15, (EndNode), VoidStamp),
-    (16, (MergeNode [7, 15] None 17), VoidStamp),
-    (17, (ReturnNode (Some 1) None), default_stamp)
-  ]"
-values "{g' . ConditionalEliminationPhase exImpliesElim (0, {}, [], []) g'}"
-
-(* same as previous but condition is in else so condition is negated -- shouldn't optimize *)
-definition exImpliesElimNeg :: "IRGraph" where
-  "exImpliesElimNeg = irgraph [
-    (0, (StartNode (None) (4)), VoidStamp),
-    (1, (ParameterNode (0)), default_stamp),
-    (2, (ParameterNode (1)), default_stamp),
-    (3, (IntegerEqualsNode (1) (2)), default_stamp),
-    (4, (IfNode (3) (6) (5)), VoidStamp),
-    (5, (BeginNode (9)), VoidStamp),
-    (6, (BeginNode (7)), VoidStamp),
-    (7, (EndNode), VoidStamp),
-    (8, (IntegerLessThanNode (1) (2)), default_stamp),
-    (9, (IfNode (8) (10) (11)), default_stamp),
-    (10, (BeginNode 12), VoidStamp),
-    (11, (BeginNode 13), VoidStamp),
-    (12, (EndNode), VoidStamp),
-    (13, (EndNode), VoidStamp),
-    (14, (MergeNode [12, 13] None 15), VoidStamp),
-    (15, (EndNode), VoidStamp),
-    (16, (MergeNode [7, 15] None 17), VoidStamp),
-    (17, (ReturnNode (Some 1) None), default_stamp)
-  ]"
-values "{g' . ConditionalEliminationPhase exImpliesElimNeg (0, {}, [], []) g'}"
-
-
-(* tests the negation implies rule *)
-definition exImpliesElimNegation :: "IRGraph" where
-  "exImpliesElimNegation = irgraph [
-    (0, (StartNode (None) (4)), VoidStamp),
-    (1, (ParameterNode (0)), default_stamp),
-    (2, (ParameterNode (1)), default_stamp),
-    (3, (IntegerEqualsNode (1) (2)), default_stamp),
-    (4, (IfNode (3) (5) (6)), VoidStamp),
-    (5, (BeginNode (9)), VoidStamp),
-    (6, (BeginNode (7)), VoidStamp),
-    (7, (EndNode), VoidStamp),
-    (8, (IntegerLessThanNode (1) (2)), default_stamp),
-    (200, (NegateNode 8), default_stamp),
-    (9, (IfNode (200) (10) (11)), default_stamp),
-    (10, (BeginNode 12), VoidStamp),
-    (11, (BeginNode 13), VoidStamp),
-    (12, (EndNode), VoidStamp),
-    (13, (EndNode), VoidStamp),
-    (14, (MergeNode [12, 13] None 15), VoidStamp),
-    (15, (EndNode), VoidStamp),
-    (16, (MergeNode [7, 15] None 17), VoidStamp),
-    (17, (ReturnNode (Some 1) None), default_stamp)
-  ]"
-values "{g' . ConditionalEliminationPhase exImpliesElimNegation (0, {}, [], []) g'}"
-
-
-definition ConditionalEliminationTest4_test2Snippet_initial :: IRGraph where
-  "ConditionalEliminationTest4_test2Snippet_initial = irgraph [
-  (0, (StartNode  (Some 3) 7), VoidStamp),
-  (1, (ParameterNode 0), IntegerStamp 32 (-2147483648) 2147483647),
-  (2, (ParameterNode 1), IntegerStamp 32 (-2147483648) 2147483647),
-  (3, (FrameState []  None None None), IllegalStamp),
-  (4, (IntegerLessThanNode 1 2), VoidStamp),
-  (5, (BeginNode 8), VoidStamp),
-  (6, (BeginNode 13), VoidStamp),
-  (7, (IfNode 4 6 5), VoidStamp),
-  (8, (EndNode), VoidStamp),
-  (9, (MergeNode  [8, 10]  (Some 16) 18), VoidStamp),
-  (10, (EndNode), VoidStamp),
-  (11, (BeginNode 15), VoidStamp),
-  (12, (BeginNode 10), VoidStamp),
-  (13, (IfNode 4 11 12), VoidStamp),
-  (14, (ConstantNode (IntVal 32 (1))), IntegerStamp 32 1 1),
-  (15, (ReturnNode  (Some 14)  None), VoidStamp),
-  (16, (FrameState []  None None None), IllegalStamp),
-  (17, (ConstantNode (IntVal 32 (2))), IntegerStamp 32 2 2),
-  (18, (ReturnNode  (Some 17)  None), VoidStamp)
-  ]"
-values "{g' . ConditionalEliminationPhase ConditionalEliminationTest4_test2Snippet_initial (0, {}, [], []) g'}"
+code_pred (modes: i \<Rightarrow> i \<Rightarrow> i \<Rightarrow> o \<Rightarrow> o \<Rightarrow> o \<Rightarrow> bool) ConditionalEliminationPhaseWithTrace .
 
 
 lemma IfNodeStepE: "g \<turnstile> (nid, m, h) \<rightarrow> (nid', m', h) \<Longrightarrow>
@@ -711,13 +629,20 @@ lemma IfNodeStepE: "g \<turnstile> (nid, m, h) \<rightarrow> (nid', m', h) \<Lon
   using StepE
   by (smt (verit, best) IfNode Pair_inject stepDet)
 
-
-lemma ifNodeHasCondEval:
+lemma ifNodeHasCondEvalStutter:
   assumes "(g m h \<turnstile> nid \<leadsto> nid')"
   assumes "kind g nid = IfNode cond t f"
   shows "\<exists> v. (g m \<turnstile> kind g cond \<mapsto> v)"
   using IfNodeStepE assms(1) assms(2)  stutter.cases
   by (smt (z3) IRNode.disc(932) IRNode.distinct(893) IRNode.distinct(913) IRNode.distinct(927) IRNode.distinct(929) IRNode.distinct(933) IRNode.distinct(947) IRNode.sel(59) StepE is_EndNode.simps(12) is_sequential_node.simps(17))
+
+lemma ifNodeHasCondEval:
+  assumes "(g \<turnstile> (nid, m, h) \<rightarrow> (nid', m', h'))"
+  assumes "kind g nid = IfNode cond t f"
+  shows "\<exists> v. (g m \<turnstile> kind g cond \<mapsto> v)"
+  using IfNodeStepE assms(1) assms(2)
+  by (smt (z3) IRNode.disc(932) IRNode.simps(938) IRNode.simps(958) IRNode.simps(972) IRNode.simps(974) IRNode.simps(978) Pair_inject StutterStep ifNodeHasCondEvalStutter isAbstractEndNodeType.simps is_EndNode.simps(12) step.cases)
+
 
 lemma replace_if_t:
   assumes "kind g nid = IfNode cond tb fb"
@@ -759,14 +684,17 @@ proof -
     using StutterStep by blast
 qed
 
-
+text \<open>
+Prove that the individual conditional elimination rules are correct
+with respect to preservation of stuttering steps.
+\<close>
 lemma ConditionalEliminationStepProof:
   assumes wg: "wff_graph g"
   assumes ws: "wff_stamps g"
   assumes nid: "nid \<in> ids g"
   assumes conds_valid: "\<forall> c \<in> conds . \<exists> v. (g m \<turnstile> c \<mapsto> v) \<and> val_to_bool v"
   assumes ce: "ConditionalEliminationStep conds stamps g nid g'"
-  
+
   shows "\<exists>nid' .(g m h \<turnstile> nid \<leadsto> nid') \<longrightarrow> (g' m h \<turnstile> nid \<leadsto> nid')"
   using ce using assms
 proof (induct g nid g' rule: ConditionalEliminationStep.induct)
@@ -776,7 +704,7 @@ proof (induct g nid g' rule: ConditionalEliminationStep.induct)
     obtain condv where condv: "g m \<turnstile> kind g cid \<mapsto> condv"
       using implies.simps impliesTrue.hyps(3) impliesTrue.prems(4)
       using impliesTrue.hyps(2) True
-      by (metis ifNodeHasCondEval impliesTrue.hyps(1))
+      by (metis ifNodeHasCondEvalStutter impliesTrue.hyps(1))
     have condvTrue: "val_to_bool condv"
       by (metis condition_implies.intros(2) condv impliesTrue.hyps(2) impliesTrue.hyps(3) impliesTrue.prems(4) implies_true_valid)
     then show ?thesis
@@ -793,7 +721,7 @@ next
   proof (cases "(g m h \<turnstile> ifcond \<leadsto> nid')")
     case True
     obtain condv where condv: "g m \<turnstile> kind g cid \<mapsto> condv"
-      using ifNodeHasCondEval impliesFalse.hyps(1)
+      using ifNodeHasCondEvalStutter impliesFalse.hyps(1)
       using True by blast
     have condvFalse: "False = val_to_bool condv"
       using conds_valid impliesFalse.hyps(3)
@@ -817,13 +745,104 @@ next
     using StutterStep constantConditionFalse by metis
 qed
 
+
+text \<open>
+Prove that the individual conditional elimination rules are correct
+with respect to finding a bisimulation between the unoptimized and optimized graphs.
+\<close>
+lemma ConditionalEliminationStepProofBisimulation:
+  assumes wff: "wff_graph g \<and> wff_stamp g stamps"
+  assumes nid: "nid \<in> ids g"
+  assumes conds_valid: "\<forall> c \<in> conds . \<exists> v. (g m \<turnstile> c \<mapsto> v) \<and> val_to_bool v"
+  assumes ce: "ConditionalEliminationStep conds stamps g nid g'"
+
+  shows "nid | g \<sim> g'"
+  using ce using assms
+proof (induct g nid g' rule: ConditionalEliminationStep.induct)
+  case (impliesTrue g ifcond cid t f cond conds g' stamps)
+  show ?case proof (cases "\<exists>h nid'. (g \<turnstile> (ifcond, m, h) \<rightarrow> (nid', m, h))")
+    case True
+    then obtain h where gstep: "g \<turnstile> (ifcond, m, h) \<rightarrow> (t, m, h)"
+      by (metis IfNode condition_implies.intros(2) ifNodeHasCondEval impliesTrue.hyps(1) impliesTrue.hyps(2) impliesTrue.hyps(3) impliesTrue.prems(3) implies_true_valid)
+    have "g' \<turnstile> (ifcond, m, h) \<rightarrow> (t, m, h)"
+      using constantConditionTrue impliesTrue.hyps(1) impliesTrue.hyps(4) by blast
+    then show ?thesis using gstep
+      by (metis stepDet strong_noop_bisimilar.intros)
+  next
+    case False
+    then have "\<not>(\<exists>m h nid'. (g' \<turnstile> (ifcond, m, h) \<rightarrow> (nid', m, h)))"
+      using impliesTrue sorry
+    then show ?thesis using False no_step_bisimulation
+      using constantConditionTrue impliesTrue.hyps(1) impliesTrue.hyps(4) by blast
+  qed
+next
+  case (impliesFalse g ifcond cid t f cond conds g' stamps)
+  show ?case proof (cases "\<exists>h nid'. (g \<turnstile> (ifcond, m, h) \<rightarrow> (nid', m, h))")
+    case True
+    then obtain h where gstep: "g \<turnstile> (ifcond, m, h) \<rightarrow> (f, m, h)"
+      by (metis IfNode condition_implies.intros(2) ifNodeHasCondEval impliesFalse.hyps(1) impliesFalse.hyps(2) impliesFalse.hyps(3) impliesFalse.prems(1) impliesFalse.prems(3) implies_false_valid)
+    have "g' \<turnstile> (ifcond, m, h) \<rightarrow> (f, m, h)"
+      using constantConditionFalse impliesFalse.hyps(1) impliesFalse.hyps(4) by blast
+    then show ?thesis using gstep
+      by (metis stepDet strong_noop_bisimilar.intros)
+  next
+    case False
+    then have "\<not>(\<exists>m h nid'. (g' \<turnstile> (ifcond, m, h) \<rightarrow> (nid', m, h)))"
+      using impliesTrue sorry
+    then show ?thesis using False no_step_bisimulation
+      using constantConditionFalse impliesFalse.hyps(1) impliesFalse.hyps(4) by blast
+  qed
+next
+  case (tryFoldTrue g ifcond cid t f cond stamps g' conds)
+  show ?case proof (cases "\<exists>h nid'. (g \<turnstile> (ifcond, m, h) \<rightarrow> (nid', m, h))")
+    case True
+    obtain val where "g m \<turnstile> kind g cid \<mapsto> val"
+      using True ifNodeHasCondEval tryFoldTrue.hyps(1) by blast
+    then have "val_to_bool val"
+      using tryFoldProofTrue tryFoldTrue.prems(1) tryFoldTrue(3) 
+      by blast
+    then obtain h where gstep: "g \<turnstile> (ifcond, m, h) \<rightarrow> (t, m, h)"
+      using True
+      by (meson IfNode \<open>g m \<turnstile> kind g cid \<mapsto> val\<close> tryFoldTrue.hyps(1))
+    have "g' \<turnstile> (ifcond, m, h) \<rightarrow> (t, m, h)"
+      using constantConditionTrue tryFoldTrue.hyps(1) tryFoldTrue.hyps(4) by presburger
+    then show ?thesis using gstep
+      by (metis stepDet strong_noop_bisimilar.intros)
+  next
+    case False
+    then have "\<not>(\<exists>m h nid'. (g' \<turnstile> (ifcond, m, h) \<rightarrow> (nid', m, h)))"
+      using impliesTrue sorry
+    then show ?thesis using False no_step_bisimulation
+      using constantConditionTrue tryFoldTrue.hyps(1) tryFoldTrue.hyps(4) by blast
+  qed
+next
+  case (tryFoldFalse g ifcond cid t f cond stamps g' conds)
+  show ?case proof (cases "\<exists>h nid'. (g \<turnstile> (ifcond, m, h) \<rightarrow> (nid', m, h))")
+    case True
+    then obtain h where gstep: "g \<turnstile> (ifcond, m, h) \<rightarrow> (f, m, h)"
+      by (meson IfNode ifNodeHasCondEval tryFoldFalse.hyps(1) tryFoldFalse.hyps(3) tryFoldFalse.prems(1) tryFoldProofFalse)
+    have "g' \<turnstile> (ifcond, m, h) \<rightarrow> (f, m, h)"
+      using constantConditionFalse tryFoldFalse.hyps(1) tryFoldFalse.hyps(4) by blast
+    then show ?thesis using gstep
+      by (metis stepDet strong_noop_bisimilar.intros)
+  next
+    case False
+    then have "\<not>(\<exists>m h nid'. (g' \<turnstile> (ifcond, m, h) \<rightarrow> (nid', m, h)))"
+      using impliesTrue sorry
+    then show ?thesis using False no_step_bisimulation
+      using constantConditionFalse tryFoldFalse.hyps(1) tryFoldFalse.hyps(4) by blast
+  qed
+qed
+
+
+text \<open>Mostly experimental proofs from here on out.\<close>
+
 (* lies we tell isabelle to get things to pass *)
 lemma if_step:
   assumes "nid \<in> ids g"
   assumes "(kind g nid) \<in> control_nodes"
   shows "(g m h \<turnstile> nid \<leadsto> nid')"
   using assms apply (cases "kind g nid") sorry
-
 
 lemma StepConditionsValid:
   assumes "\<forall> cond \<in> set conds. (g m \<turnstile> cond \<mapsto> v) \<and> val_to_bool v"
@@ -851,7 +870,6 @@ case (3)
     using assms(1) by force
 qed
 
-
 lemma ConditionalEliminationPhaseProof:
   assumes "wff_graph g"
   assumes "wff_stamps g"
@@ -876,49 +894,6 @@ next
   case (4)
   then show ?case sorry
 qed
-qed
-
-
-lemma replaceUsagesFoldAlwaysDistinct:
-  assumes wff: "wff_graph g \<and> wff_stamps g"
-  assumes ifkind: "kind g ifcond = (IfNode cond t f)"
-  assumes condkind: "kind g cond = (IntegerEqualsNode x y)"
-  assumes condeval: "g m \<turnstile> kind g cond \<mapsto> v"
-  assumes ran: "alwaysDistinct (stamp g x) (stamp g y)"
-  assumes g': "g' = replace_usages ifcond f g"
-  shows "\<exists>nid' .(g m h \<turnstile> ifcond \<leadsto> nid') \<longleftrightarrow> (g' m h \<turnstile> ifcond \<leadsto> nid')"
-proof -
-  have "v = IntVal 1 0"
-    using tryFoldIntegerEqualsAlwaysDistinct
-    using condeval condkind ran wff by blast
-  then have g1step: "g \<turnstile> (ifcond, m, h) \<rightarrow> (f, m, h)"
-    by (metis IfNode condeval ifkind val_to_bool.simps(1))
-  have g2step: "g' \<turnstile> (ifcond, m, h) \<rightarrow> (f, m, h)"
-    using g' unfolding replace_usages.simps
-    by (simp add: step.RefNode)
-  from g1step g2step show ?thesis
-    using StutterStep by meson
-qed
-
-lemma replaceUsagesFoldNeverDistinct:
-  assumes wff: "wff_graph g \<and> wff_stamps g"
-  assumes ifkind: "kind g ifcond = (IfNode cond t f)"
-  assumes condkind: "kind g cond = (IntegerEqualsNode x y)"
-  assumes condeval: "g m \<turnstile> kind g cond \<mapsto> v"
-  assumes ran: "neverDistinct (stamp g x) (stamp g y)"
-  assumes g': "g' = replace_usages ifcond t g"
-  shows "\<exists>nid' .(g m h \<turnstile> ifcond \<leadsto> nid') \<longleftrightarrow> (g' m h \<turnstile> ifcond \<leadsto> nid')"
-proof -
-  have "v = IntVal 1 1"
-    using tryFoldIntegerEqualsNeverDistinct
-    using condeval condkind ran wff by blast
-  then have g1step: "g \<turnstile> (ifcond, m, h) \<rightarrow> (t, m, h)"
-    by (smt IfNode condeval ifkind val_to_bool.simps(1))
-  have g2step: "g' \<turnstile> (ifcond, m, h) \<rightarrow> (t, m, h)"
-    using g' unfolding replace_usages.simps
-    by (simp add: step.RefNode)
-  from g1step g2step show ?thesis
-    using StutterStep by blast
 qed
 
 end
