Tests/ConditionalEliminationSyntheticTests.thy
@@ -1,0 +1,207 @@
+subsection \<open>Synthetic\<close>
+
+theory
+  ConditionalEliminationSyntheticTests
+imports
+  Optimizations.ConditionalElimination
+begin
+
+text \<open>
+Synthetic optimization cases (written by hand during the development of the phase)
+which are useful to ensure continued correctness.
+
+Once the predicate compiler can be successfully defeated, these will ideally become
+regression tests that will be automatically checked during building.
+\<close>
+
+definition ConditionalEliminationTest1_test1Snippet_initial :: IRGraph where
+  "ConditionalEliminationTest1_test1Snippet_initial = irgraph [
+  (0, (StartNode  (Some 2) 7), VoidStamp),
+  (1, (ParameterNode 0), IntegerStamp 32 (-2147483648) (2147483647)),
+  (2, (FrameState []  None None None), IllegalStamp),
+  (3, (ConstantNode (IntVal 32 (0))), IntegerStamp 32 (0) (0)),
+  (4, (IntegerEqualsNode 1 3), VoidStamp),
+  (5, (BeginNode 39), VoidStamp),
+  (6, (BeginNode 12), VoidStamp),
+  (7, (IfNode 4 6 5), VoidStamp),
+  (8, (ConstantNode (IntVal 32 (5))), IntegerStamp 32 (5) (5)),
+  (9, (IntegerEqualsNode 1 8), VoidStamp),
+  (10, (BeginNode 16), VoidStamp),
+  (11, (BeginNode 14), VoidStamp),
+  (12, (IfNode 9 11 10), VoidStamp),
+  (13, (ConstantNode (IntVal 32 (100))), IntegerStamp 32 (100) (100)),
+  (14, (StoreFieldNode 14 ''org.graalvm.compiler.core.test.ConditionalEliminationTestBase::sink2'' 13  (Some 15)  None 18), VoidStamp),
+  (15, (FrameState []  None None None), IllegalStamp),
+  (16, (EndNode), VoidStamp),
+  (17, (MergeNode  [16, 18]  (Some 19) 24), VoidStamp),
+  (18, (EndNode), VoidStamp),
+  (19, (FrameState []  None None None), IllegalStamp),
+  (20, (ConstantNode (IntVal 32 (101))), IntegerStamp 32 (101) (101)),
+  (21, (IntegerLessThanNode 1 20), VoidStamp),
+  (22, (BeginNode 30), VoidStamp),
+  (23, (BeginNode 25), VoidStamp),
+  (24, (IfNode 21 23 22), VoidStamp),
+  (25, (EndNode), VoidStamp),
+  (26, (MergeNode  [25, 27, 34]  (Some 35) 43), VoidStamp),
+  (27, (EndNode), VoidStamp),
+  (28, (BeginNode 32), VoidStamp),
+  (29, (BeginNode 27), VoidStamp),
+  (30, (IfNode 4 28 29), VoidStamp),
+  (31, (ConstantNode (IntVal 32 (200))), IntegerStamp 32 (200) (200)),
+  (32, (StoreFieldNode 32 ''org.graalvm.compiler.core.test.ConditionalEliminationTest1::sink3'' 31  (Some 33)  None 34), VoidStamp),
+  (33, (FrameState []  None None None), IllegalStamp),
+  (34, (EndNode), VoidStamp),
+  (35, (FrameState []  None None None), IllegalStamp),
+  (36, (ConstantNode (IntVal 32 (2))), IntegerStamp 32 (2) (2)),
+  (37, (IntegerEqualsNode 1 36), VoidStamp),
+  (38, (BeginNode 45), VoidStamp),
+  (39, (EndNode), VoidStamp),
+  (40, (MergeNode  [39, 41, 47]  (Some 48) 49), VoidStamp),
+  (41, (EndNode), VoidStamp),
+  (42, (BeginNode 41), VoidStamp),
+  (43, (IfNode 37 42 38), VoidStamp),
+  (44, (ConstantNode (IntVal 32 (1))), IntegerStamp 32 (1) (1)),
+  (45, (StoreFieldNode 45 ''org.graalvm.compiler.core.test.ConditionalEliminationTestBase::sink1'' 44  (Some 46)  None 47), VoidStamp),
+  (46, (FrameState []  None None None), IllegalStamp),
+  (47, (EndNode), VoidStamp),
+  (48, (FrameState []  None None None), IllegalStamp),
+  (49, (StoreFieldNode 49 ''org.graalvm.compiler.core.test.ConditionalEliminationTestBase::sink0'' 3  (Some 50)  None 51), VoidStamp),
+  (50, (FrameState []  None None None), IllegalStamp),
+  (51, (ReturnNode  None  None), VoidStamp)
+  ]"
+values "{g' . ConditionalEliminationPhase ConditionalEliminationTest1_test1Snippet_initial (0, {}, [], []) g'}"
+
+
+definition exAlwaysDistinct :: "IRGraph" where
+  "exAlwaysDistinct = irgraph [
+    (0, (StartNode (None) (4)), VoidStamp),
+    (1, (ParameterNode (0)), IntegerStamp 32 (1) (2)),
+    (2, (ParameterNode (1)), IntegerStamp 32 (3) (4)),
+    (3, (IntegerEqualsNode (1) (2)), default_stamp),
+    (4, (IfNode (3) (5) (6)), VoidStamp),
+    (5, (BeginNode 7), VoidStamp),
+    (6, (BeginNode 8), VoidStamp),
+    (7, (EndNode), VoidStamp),
+    (8, (EndNode), VoidStamp),
+    (9, (MergeNode [7, 8] None 11), VoidStamp),
+    (10, (ValuePhiNode 10 [1, 2] 9), VoidStamp),
+    (11, (ReturnNode ((Some 10)) (None)), default_stamp)]"
+
+values "{g' . ConditionalEliminationPhase exAlwaysDistinct (0, {}, [], []) g'}"
+
+
+definition exNeverDistinct :: "IRGraph" where
+  "exNeverDistinct = irgraph [
+    (0, (StartNode (None) (4)), VoidStamp),
+    (1, (ParameterNode (0)), IntegerStamp 32 (1) (1)),
+    (2, (ParameterNode (1)), IntegerStamp 32 (1) (1)),
+    (3, (IntegerEqualsNode (1) (2)), default_stamp),
+    (4, (IfNode (3) (5) (6)), VoidStamp),
+    (5, (BeginNode 7), VoidStamp),
+    (6, (BeginNode 8), VoidStamp),
+    (7, (EndNode), VoidStamp),
+    (8, (EndNode), VoidStamp),
+    (9, (MergeNode [7, 8] None 11), VoidStamp),
+    (10, (ValuePhiNode 10 [1, 2] 9), VoidStamp),
+    (11, (ReturnNode ((Some 10)) (None)), default_stamp)]"
+values "{g' . ConditionalEliminationPhase exNeverDistinct (0, {}, [], []) g'}"
+
+definition exImpliesElim :: "IRGraph" where
+  "exImpliesElim = irgraph [
+    (0, (StartNode (None) (4)), VoidStamp),
+    (1, (ParameterNode (0)), default_stamp),
+    (2, (ParameterNode (1)), default_stamp),
+    (3, (IntegerEqualsNode (1) (2)), default_stamp),
+    (4, (IfNode (3) (5) (6)), VoidStamp),
+    (5, (BeginNode (9)), VoidStamp),
+    (6, (BeginNode (7)), VoidStamp),
+    (7, (EndNode), VoidStamp),
+    (8, (IntegerLessThanNode (1) (2)), default_stamp),
+    (9, (IfNode (8) (10) (11)), default_stamp),
+    (10, (BeginNode 12), VoidStamp),
+    (11, (BeginNode 13), VoidStamp),
+    (12, (EndNode), VoidStamp),
+    (13, (EndNode), VoidStamp),
+    (14, (MergeNode [12, 13] None 15), VoidStamp),
+    (15, (EndNode), VoidStamp),
+    (16, (MergeNode [7, 15] None 17), VoidStamp),
+    (17, (ReturnNode (Some 1) None), default_stamp)
+  ]"
+values "{g' . ConditionalEliminationPhase exImpliesElim (0, {}, [], []) g'}"
+
+(* same as previous but condition is in else so condition is negated -- shouldn't optimize *)
+definition exImpliesElimNeg :: "IRGraph" where
+  "exImpliesElimNeg = irgraph [
+    (0, (StartNode (None) (4)), VoidStamp),
+    (1, (ParameterNode (0)), default_stamp),
+    (2, (ParameterNode (1)), default_stamp),
+    (3, (IntegerEqualsNode (1) (2)), default_stamp),
+    (4, (IfNode (3) (6) (5)), VoidStamp),
+    (5, (BeginNode (9)), VoidStamp),
+    (6, (BeginNode (7)), VoidStamp),
+    (7, (EndNode), VoidStamp),
+    (8, (IntegerLessThanNode (1) (2)), default_stamp),
+    (9, (IfNode (8) (10) (11)), default_stamp),
+    (10, (BeginNode 12), VoidStamp),
+    (11, (BeginNode 13), VoidStamp),
+    (12, (EndNode), VoidStamp),
+    (13, (EndNode), VoidStamp),
+    (14, (MergeNode [12, 13] None 15), VoidStamp),
+    (15, (EndNode), VoidStamp),
+    (16, (MergeNode [7, 15] None 17), VoidStamp),
+    (17, (ReturnNode (Some 1) None), default_stamp)
+  ]"
+values "{g' . ConditionalEliminationPhase exImpliesElimNeg (0, {}, [], []) g'}"
+
+
+(* tests the negation implies rule *)
+definition exImpliesElimNegation :: "IRGraph" where
+  "exImpliesElimNegation = irgraph [
+    (0, (StartNode (None) (4)), VoidStamp),
+    (1, (ParameterNode (0)), default_stamp),
+    (2, (ParameterNode (1)), default_stamp),
+    (3, (IntegerEqualsNode (1) (2)), default_stamp),
+    (4, (IfNode (3) (5) (6)), VoidStamp),
+    (5, (BeginNode (9)), VoidStamp),
+    (6, (BeginNode (7)), VoidStamp),
+    (7, (EndNode), VoidStamp),
+    (8, (IntegerLessThanNode (1) (2)), default_stamp),
+    (200, (NegateNode 8), default_stamp),
+    (9, (IfNode (200) (10) (11)), default_stamp),
+    (10, (BeginNode 12), VoidStamp),
+    (11, (BeginNode 13), VoidStamp),
+    (12, (EndNode), VoidStamp),
+    (13, (EndNode), VoidStamp),
+    (14, (MergeNode [12, 13] None 15), VoidStamp),
+    (15, (EndNode), VoidStamp),
+    (16, (MergeNode [7, 15] None 17), VoidStamp),
+    (17, (ReturnNode (Some 1) None), default_stamp)
+  ]"
+values "{g' . ConditionalEliminationPhase exImpliesElimNegation (0, {}, [], []) g'}"
+
+
+definition ConditionalEliminationTest4_test2Snippet_initial :: IRGraph where
+  "ConditionalEliminationTest4_test2Snippet_initial = irgraph [
+  (0, (StartNode  (Some 3) 7), VoidStamp),
+  (1, (ParameterNode 0), IntegerStamp 32 (-2147483648) 2147483647),
+  (2, (ParameterNode 1), IntegerStamp 32 (-2147483648) 2147483647),
+  (3, (FrameState []  None None None), IllegalStamp),
+  (4, (IntegerLessThanNode 1 2), VoidStamp),
+  (5, (BeginNode 8), VoidStamp),
+  (6, (BeginNode 13), VoidStamp),
+  (7, (IfNode 4 6 5), VoidStamp),
+  (8, (EndNode), VoidStamp),
+  (9, (MergeNode  [8, 10]  (Some 16) 18), VoidStamp),
+  (10, (EndNode), VoidStamp),
+  (11, (BeginNode 15), VoidStamp),
+  (12, (BeginNode 10), VoidStamp),
+  (13, (IfNode 4 11 12), VoidStamp),
+  (14, (ConstantNode (IntVal 32 (1))), IntegerStamp 32 1 1),
+  (15, (ReturnNode  (Some 14)  None), VoidStamp),
+  (16, (FrameState []  None None None), IllegalStamp),
+  (17, (ConstantNode (IntVal 32 (2))), IntegerStamp 32 2 2),
+  (18, (ReturnNode  (Some 17)  None), VoidStamp)
+  ]"
+values "{g' . ConditionalEliminationPhase ConditionalEliminationTest4_test2Snippet_initial (0, {}, [], []) g'}"
+
+end
